concurrency/Modular/implementations4/giveup_ds.h
@@ -1,0 +1,4 @@
+#include "giveup_template.h"
+
+void insertOp_giveup(css *c, node *p, int x, void *value, Status status);
+void printDS_giveup(css *t);
