concurrency/Modular/implementations4_Mac/giveup_template.h
@@ -1,0 +1,48 @@
+#include "data_structure.h"
+#include "template.h"
+
+typedef struct md_entry { lock_t *lock; int min; int max; } md_entry;
+typedef struct css { node* root; md_entry* metadata[16384]; } css;
+
+int hash(node* p);
+
+int inRange(md_entry* m, int x);
+md_entry* lookup_md(css* c, node* p);
+Status traverse(css* c, pn *pn, int x);
+
+void insertOp_giveup(css* c, node *p, int x, void* value, Status status);
+void insertOp_helper(css* c, node *p, int x, void* value, Status status);
+
+void change_value_helper(node* p_ds, void* value);
+void *get_value_helper(node* p);
+
+//support print ds
+void printDS_giveup (css *t);
+void printDS_helper (css *t);
+
+typedef struct stack {
+    struct node * items[100]; // Assuming a maximum of 100 nodes
+    int top;
+} stack;
+
+static void initStack(stack* s) {
+    s->top = -1;
+}
+
+// Function to push a node onto the stack
+static void push(stack* s, node * item) {
+    s->items[++s->top] = item;
+}
+
+// Function to check if the stack is empty
+static int isEmpty(stack* s) {
+    return s->top == -1;
+}
+
+// Function to pop a node from the stack
+static node* pop(stack* s) {
+    if (!isEmpty(s)) {
+        return s->items[s->top--];
+    }
+    return NULL;
+}
