concurrency/Modular/implementations4_Mac/list.c
@@ -1,0 +1,74 @@
+#include "data_structure.h"
+
+typedef struct node { int key; void *value; node *next; } node;
+
+Status findNext(node* p, void** n_list, int x) {
+    int y = p->key;
+    if (x > y) {
+        *n_list = p->next;
+        return CONTINUE;
+    }
+    else if (x < y) {
+        return NOTFOUND;
+    }
+    else {
+        return FOUND;
+    }
+}
+
+node * insertOp(node* p, int x, void* value, int *signal){
+    node* new_node = surely_malloc(sizeof(node));
+    new_node->key = x;
+    new_node->value = value;
+    new_node->next = NULL;
+
+    // If the current node is NULL, place the new node here
+    if(p == NULL){
+        return new_node;
+    }
+
+    // Determine whether to insert to the right or in the middle 
+    if(x < p->key){
+        new_node->next = p->next;
+        p->next = new_node;
+        // Swap keys and values with the new node
+        int temp_key = p->key;
+        p->key = x;
+        new_node->key = temp_key;
+        
+        void* temp_value = p->value;
+        p->value = value;
+        new_node->value = temp_value;
+        
+        *signal = 0; // Inserted in the middle
+    }
+    else{
+        // Insert after p
+        new_node->next = p->next;
+        p->next = new_node;
+        *signal = 1; // Inserted to the right
+    }
+    return new_node;
+}
+
+void change_value(node* p, void* value){
+    p->value = value;
+}
+
+void* get_value(node* p){
+    return p->value;
+}
+
+int get_key(node* p){
+    return p->key;
+}
+
+void *get_next(node *node) {
+    if (node == NULL)
+        return NULL; 
+    return node->next;
+}
+
+void print_key_value(node *node){
+    printf ("(%d, %s) \n", node->key, (char*)node->value);
+}
