concurrency/Modular/implementations4_Mac/list_lock.c
@@ -1,0 +1,44 @@
+#include "lock_ds.h"
+
+void insertOp_lock(css *c, node *p, int x, void *value, Status status){
+    int signal; // Indicates left, right, or NULL
+    node *new_node = insertOp(p, x, value, &signal);
+
+    // Calculate index and allocate metadata for the new node
+    int idx = hash(new_node);
+    c->metadata[idx] = surely_malloc(sizeof(md_entry));
+
+    // Initialize lock for the new node
+    lock_t* lock = surely_malloc(sizeof(lock_t));
+    makelock(lock);
+    c->metadata[idx]->lock = lock;
+    release(lock);
+
+    // Update root and metadata if status is CONTINUE
+    if (status == CONTINUE) {
+        c->root = new_node;
+        return;
+    }
+}
+
+void printDS_lock(css *t){
+    printf("For Linked list - LOCK-COUPLING\n");
+    struct node* tgt;
+    tgt = get_root(t);
+
+    if (tgt == NULL) {
+        return;
+    }
+    stack s;
+    initStack(&s);
+    node * current = tgt;
+
+    while (current != NULL){
+        push(&s, current);
+        current = (node*)get_next(current);
+    }
+    while (!isEmpty(&s)){   
+        current = pop(&s);
+        print_key_value(current);
+    }
+}
