concurrency/Modular/implementations4_Mac/lock_ds.h
@@ -1,0 +1,4 @@
+#include "lock_template.h"
+
+void insertOp_lock(css* c, node *p, int x, void* value, Status status);
+void printDS_lock(css *t);
