concurrency/Modular/implementations4_Mac/lock_template.c
@@ -1,17 +1,10 @@
-#include "giveup_template.h"
+#include "lock_template.h"
 
 
 int hash(node* p) {
     // Ensure the pointer is cast to a proper unsigned type before multiplication
     uintptr_t ptr_value = (uintptr_t)p;
     return (int)(ptr_value * 654435761ULL % TABLE_SIZE);
-}
-
-int inRange(md_entry* m, int x){
-    if (x > m->min && x < m->max)
-        return 1;
-    else
-        return 0;
 }
 
 md_entry* lookup_md(css* c, node* p){
@@ -22,34 +15,33 @@ md_entry* lookup_md(css* c, node* p){
 Status traverse(css* c, pn *pn, int x) {
     Status status = NOTFOUND;
     if(!pn->n) return CONTINUE; // special case for empty data structure
-    node* p = pn->n;
+    md_entry* md_n = lookup_md(c, pn->n);
+    md_entry* md_p;
+    acquire(md_n->lock); 
     for( ; ; ){
-        if(!pn->n) return NOTFOUND;
-        md_entry* md = lookup_md(c, pn->n);
-        acquire(md->lock);
         pn->p = pn->n;
-        if (inRange (md, x) == 1){
-            status = findNext(pn->p, (void**)&pn->n, x);
-            if (status == FOUND){
-                break;
-            }
-            else if (status == NOTFOUND){
-                break;
-            }
-            else{
-                release(md->lock);
-            }
+        status = findNext(pn->p, (void**)&pn->n, x);
+        if(!pn->n) {
+            return NOTFOUND;
+        }
+        if (status == FOUND){
+            break;
+        }
+        else if (status == NOTFOUND){
+            break;
         }
         else{
-            release(md->lock);
-            pn->n = p;
+            md_n = lookup_md(c, pn->n);
+            md_p = lookup_md(c, pn->p);
+            acquire(md_n->lock); //acquire pn->n
+            release(md_p->lock); // release pn->p
         }
     }
     return status;
 }
 
 void insertOp_helper(css* c, node *p, int x, void* value, Status status){
-    insertOp_giveup(c, p, x, value, status);
+    insertOp_lock(c, p, x, value, status);
 }
 
 css* make_css(){
@@ -58,7 +50,7 @@ css* make_css(){
     return new_css;
 }
 
-lock_t get_lock(css* c, node* p){
+lock_t * get_lock(css* c, node* p){
     md_entry* m = lookup_md(c, p);
     fflush(stdout);
     return m->lock;
@@ -79,5 +71,5 @@ void *get_value_helper(node* p){
 //for BST
 
 void printDS_helper (css *t){
-    printDS_giveup(t);
+    printDS_lock(t);
 }
