concurrency/Modular/implementations_Mac/list_lock.c
@@ -3,7 +3,7 @@
 void insertOp_lock(node_t* p, int x, void* value, Status status){
     DList dlist; 
     dlist.size = 1; // For Linked-list 
-    dlist.list = (void**)surely_malloc(dlist.size * sizeof(node_t));
+    dlist.list = (void**)surely_malloc(dlist.size * sizeof(node_t*));
     dlist.list[0] = (struct node_t*)surely_malloc(sizeof (node_t));
     if (status == NULLNEXT) {
         ((node_t*)dlist.list[0])->t = NULL;
@@ -19,8 +19,10 @@ void insertOp_lock(node_t* p, int x, void* value, Status status){
         ((node_t*)dlist.list[0])->lock = l;
         release(l);
         ((node_t*)dlist.list[0])->t = p->t;
+        p->t = NULL;
         insertOp(&(p->t), x, value, status, &dlist);
     }
+    free(dlist.list);
 } 
 
 void printDS_lock(void **t){
