concurrency/Modular/implementations_Mac/main.c
@@ -17,9 +17,9 @@ void *thread_func(void *args) {
     lock_t *l = &thread_lock;
     
     // insert at key 1
-    insert(tb,6,"ONE_FROM_THREAD");
-    insert(tb,4,"FOUR");
-    insert(tb,5,"FIVE");
+    insert(tb,10,"ten");
+    //insert(tb,4,"FOUR");
+    //insert(tb,5,"FIVE");
     
     release((void*)l);
     return (void *)NULL;
@@ -31,16 +31,15 @@ int main (void) {
     //lock_t *t_lock ;
     lock_t *t_lock = &thread_lock;
     insert(tb,3,"three");
+    insert(tb,5,"five");
     insert(tb,2,"two");
-    insert(tb,1,"One");
-    insert(tb,6,"four");
     
     //t_lock = makelock();
     makelock((void*)t_lock);
     // Spawn
     spawn((void *)&thread_func, (void *)t_lock);
     // JOIN
-    insert(tb,6,"six");
+    //insert(tb,6,"six");
     acquire((void*)t_lock);
     freelock((void*)t_lock);
     printf ("\nTraverse\n");
