concurrency/Modular/templates/.Makefile.coq.d
@@ -1,0 +1,6 @@
+flows_ora.vo flows_ora.glob flows_ora.v.beautified flows_ora.required_vo: flows_ora.v 
+flows_ora.vio: flows_ora.v 
+flows_ora.vos flows_ora.vok flows_ora.required_vos: flows_ora.v 
+puretree.vo puretree.glob puretree.v.beautified puretree.required_vo: puretree.v 
+puretree.vio: puretree.v 
+puretree.vos puretree.vok puretree.required_vos: puretree.v 
