concurrency/Modular/implementations/list_giveup.v
@@ -1,0 +1,1047 @@
+From Coq Require Import String List ZArith.
+From compcert Require Import Coqlib Integers Floats AST Ctypes Cop Clight Clightdefs.
+Import Clightdefs.ClightNotations.
+Local Open Scope Z_scope.
+Local Open Scope string_scope.
+Local Open Scope clight_scope.
+
+Module Info.
+  Definition version := "3.12".
+  Definition build_number := "".
+  Definition build_tag := "".
+  Definition build_branch := "".
+  Definition arch := "aarch64".
+  Definition model := "default".
+  Definition abi := "apple".
+  Definition bitsize := 64.
+  Definition big_endian := false.
+  Definition source_file := "list_giveup.c".
+  Definition normalized := true.
+End Info.
+
+Definition _DList : ident := $"DList".
+Definition ___builtin_annot : ident := $"__builtin_annot".
+Definition ___builtin_annot_intval : ident := $"__builtin_annot_intval".
+Definition ___builtin_bswap : ident := $"__builtin_bswap".
+Definition ___builtin_bswap16 : ident := $"__builtin_bswap16".
+Definition ___builtin_bswap32 : ident := $"__builtin_bswap32".
+Definition ___builtin_bswap64 : ident := $"__builtin_bswap64".
+Definition ___builtin_cls : ident := $"__builtin_cls".
+Definition ___builtin_clsl : ident := $"__builtin_clsl".
+Definition ___builtin_clsll : ident := $"__builtin_clsll".
+Definition ___builtin_clz : ident := $"__builtin_clz".
+Definition ___builtin_clzl : ident := $"__builtin_clzl".
+Definition ___builtin_clzll : ident := $"__builtin_clzll".
+Definition ___builtin_ctz : ident := $"__builtin_ctz".
+Definition ___builtin_ctzl : ident := $"__builtin_ctzl".
+Definition ___builtin_ctzll : ident := $"__builtin_ctzll".
+Definition ___builtin_debug : ident := $"__builtin_debug".
+Definition ___builtin_expect : ident := $"__builtin_expect".
+Definition ___builtin_fabs : ident := $"__builtin_fabs".
+Definition ___builtin_fabsf : ident := $"__builtin_fabsf".
+Definition ___builtin_fence : ident := $"__builtin_fence".
+Definition ___builtin_fmadd : ident := $"__builtin_fmadd".
+Definition ___builtin_fmax : ident := $"__builtin_fmax".
+Definition ___builtin_fmin : ident := $"__builtin_fmin".
+Definition ___builtin_fmsub : ident := $"__builtin_fmsub".
+Definition ___builtin_fnmadd : ident := $"__builtin_fnmadd".
+Definition ___builtin_fnmsub : ident := $"__builtin_fnmsub".
+Definition ___builtin_fsqrt : ident := $"__builtin_fsqrt".
+Definition ___builtin_membar : ident := $"__builtin_membar".
+Definition ___builtin_memcpy_aligned : ident := $"__builtin_memcpy_aligned".
+Definition ___builtin_sel : ident := $"__builtin_sel".
+Definition ___builtin_sqrt : ident := $"__builtin_sqrt".
+Definition ___builtin_unreachable : ident := $"__builtin_unreachable".
+Definition ___builtin_va_arg : ident := $"__builtin_va_arg".
+Definition ___builtin_va_copy : ident := $"__builtin_va_copy".
+Definition ___builtin_va_end : ident := $"__builtin_va_end".
+Definition ___builtin_va_start : ident := $"__builtin_va_start".
+Definition ___compcert_i64_dtos : ident := $"__compcert_i64_dtos".
+Definition ___compcert_i64_dtou : ident := $"__compcert_i64_dtou".
+Definition ___compcert_i64_sar : ident := $"__compcert_i64_sar".
+Definition ___compcert_i64_sdiv : ident := $"__compcert_i64_sdiv".
+Definition ___compcert_i64_shl : ident := $"__compcert_i64_shl".
+Definition ___compcert_i64_shr : ident := $"__compcert_i64_shr".
+Definition ___compcert_i64_smod : ident := $"__compcert_i64_smod".
+Definition ___compcert_i64_smulh : ident := $"__compcert_i64_smulh".
+Definition ___compcert_i64_stod : ident := $"__compcert_i64_stod".
+Definition ___compcert_i64_stof : ident := $"__compcert_i64_stof".
+Definition ___compcert_i64_udiv : ident := $"__compcert_i64_udiv".
+Definition ___compcert_i64_umod : ident := $"__compcert_i64_umod".
+Definition ___compcert_i64_umulh : ident := $"__compcert_i64_umulh".
+Definition ___compcert_i64_utod : ident := $"__compcert_i64_utod".
+Definition ___compcert_i64_utof : ident := $"__compcert_i64_utof".
+Definition ___compcert_va_composite : ident := $"__compcert_va_composite".
+Definition ___compcert_va_float64 : ident := $"__compcert_va_float64".
+Definition ___compcert_va_int32 : ident := $"__compcert_va_int32".
+Definition ___compcert_va_int64 : ident := $"__compcert_va_int64".
+Definition ___stringlit_1 : ident := $"__stringlit_1".
+Definition _atom_int : ident := $"atom_int".
+Definition _current : ident := $"current".
+Definition _dlist : ident := $"dlist".
+Definition _exit : ident := $"exit".
+Definition _free : ident := $"free".
+Definition _getNext : ident := $"getNext".
+Definition _initStack : ident := $"initStack".
+Definition _insertOp : ident := $"insertOp".
+Definition _insertOp_giveup : ident := $"insertOp_giveup".
+Definition _isEmpty : ident := $"isEmpty".
+Definition _item : ident := $"item".
+Definition _items : ident := $"items".
+Definition _l : ident := $"l".
+Definition _list : ident := $"list".
+Definition _lock : ident := $"lock".
+Definition _main : ident := $"main".
+Definition _makelock : ident := $"makelock".
+Definition _malloc : ident := $"malloc".
+Definition _max : ident := $"max".
+Definition _min : ident := $"min".
+Definition _n : ident := $"n".
+Definition _node : ident := $"node".
+Definition _node_t : ident := $"node_t".
+Definition _p : ident := $"p".
+Definition _pop : ident := $"pop".
+Definition _printDS_giveup : ident := $"printDS_giveup".
+Definition _printKey : ident := $"printKey".
+Definition _printf : ident := $"printf".
+Definition _push : ident := $"push".
+Definition _release : ident := $"release".
+Definition _s : ident := $"s".
+Definition _size : ident := $"size".
+Definition _stack : ident := $"stack".
+Definition _status : ident := $"status".
+Definition _surely_malloc : ident := $"surely_malloc".
+Definition _t : ident := $"t".
+Definition _tb : ident := $"tb".
+Definition _tgt : ident := $"tgt".
+Definition _thread_lock : ident := $"thread_lock".
+Definition _top : ident := $"top".
+Definition _value : ident := $"value".
+Definition _x : ident := $"x".
+Definition _t'1 : ident := 128%positive.
+Definition _t'10 : ident := 137%positive.
+Definition _t'11 : ident := 138%positive.
+Definition _t'12 : ident := 139%positive.
+Definition _t'13 : ident := 140%positive.
+Definition _t'14 : ident := 141%positive.
+Definition _t'15 : ident := 142%positive.
+Definition _t'16 : ident := 143%positive.
+Definition _t'17 : ident := 144%positive.
+Definition _t'18 : ident := 145%positive.
+Definition _t'19 : ident := 146%positive.
+Definition _t'2 : ident := 129%positive.
+Definition _t'20 : ident := 147%positive.
+Definition _t'21 : ident := 148%positive.
+Definition _t'22 : ident := 149%positive.
+Definition _t'3 : ident := 130%positive.
+Definition _t'4 : ident := 131%positive.
+Definition _t'5 : ident := 132%positive.
+Definition _t'6 : ident := 133%positive.
+Definition _t'7 : ident := 134%positive.
+Definition _t'8 : ident := 135%positive.
+Definition _t'9 : ident := 136%positive.
+
+Definition v___stringlit_1 := {|
+  gvar_info := (tarray tschar 26);
+  gvar_init := (Init_int8 (Int.repr 70) :: Init_int8 (Int.repr 111) ::
+                Init_int8 (Int.repr 114) :: Init_int8 (Int.repr 32) ::
+                Init_int8 (Int.repr 76) :: Init_int8 (Int.repr 105) ::
+                Init_int8 (Int.repr 110) :: Init_int8 (Int.repr 107) ::
+                Init_int8 (Int.repr 101) :: Init_int8 (Int.repr 100) ::
+                Init_int8 (Int.repr 45) :: Init_int8 (Int.repr 108) ::
+                Init_int8 (Int.repr 105) :: Init_int8 (Int.repr 115) ::
+                Init_int8 (Int.repr 116) :: Init_int8 (Int.repr 32) ::
+                Init_int8 (Int.repr 45) :: Init_int8 (Int.repr 32) ::
+                Init_int8 (Int.repr 71) :: Init_int8 (Int.repr 73) ::
+                Init_int8 (Int.repr 86) :: Init_int8 (Int.repr 69) ::
+                Init_int8 (Int.repr 85) :: Init_int8 (Int.repr 80) ::
+                Init_int8 (Int.repr 10) :: Init_int8 (Int.repr 0) :: nil);
+  gvar_readonly := true;
+  gvar_volatile := false
+|}.
+
+Definition v_thread_lock := {|
+  gvar_info := (tptr (Tstruct _atom_int noattr));
+  gvar_init := (Init_space 8 :: nil);
+  gvar_readonly := false;
+  gvar_volatile := false
+|}.
+
+Definition f_surely_malloc := {|
+  fn_return := (tptr tvoid);
+  fn_callconv := cc_default;
+  fn_params := ((_n, tulong) :: nil);
+  fn_vars := nil;
+  fn_temps := ((_p, (tptr tvoid)) :: (_t'1, (tptr tvoid)) :: nil);
+  fn_body :=
+(Ssequence
+  (Ssequence
+    (Scall (Some _t'1)
+      (Evar _malloc (Tfunction (Tcons tulong Tnil) (tptr tvoid) cc_default))
+      ((Etempvar _n tulong) :: nil))
+    (Sset _p (Etempvar _t'1 (tptr tvoid))))
+  (Ssequence
+    (Sifthenelse (Eunop Onotbool (Etempvar _p (tptr tvoid)) tint)
+      (Scall None (Evar _exit (Tfunction (Tcons tint Tnil) tvoid cc_default))
+        ((Econst_int (Int.repr 1) tint) :: nil))
+      Sskip)
+    (Sreturn (Some (Etempvar _p (tptr tvoid))))))
+|}.
+
+Definition v_tb := {|
+  gvar_info := (tptr (tptr (Tstruct _node_t noattr)));
+  gvar_init := (Init_space 8 :: nil);
+  gvar_readonly := false;
+  gvar_volatile := false
+|}.
+
+Definition f_initStack := {|
+  fn_return := tvoid;
+  fn_callconv := cc_default;
+  fn_params := ((_s, (tptr (Tstruct _stack noattr))) :: nil);
+  fn_vars := nil;
+  fn_temps := nil;
+  fn_body :=
+(Sassign
+  (Efield
+    (Ederef (Etempvar _s (tptr (Tstruct _stack noattr)))
+      (Tstruct _stack noattr)) _top tint)
+  (Eunop Oneg (Econst_int (Int.repr 1) tint) tint))
+|}.
+
+Definition f_push := {|
+  fn_return := tvoid;
+  fn_callconv := cc_default;
+  fn_params := ((_s, (tptr (Tstruct _stack noattr))) ::
+                (_item, (tptr (Tstruct _node_t noattr))) :: nil);
+  fn_vars := nil;
+  fn_temps := ((_t'1, tint) :: (_t'2, tint) :: nil);
+  fn_body :=
+(Ssequence
+  (Ssequence
+    (Ssequence
+      (Sset _t'2
+        (Efield
+          (Ederef (Etempvar _s (tptr (Tstruct _stack noattr)))
+            (Tstruct _stack noattr)) _top tint))
+      (Sset _t'1
+        (Ecast
+          (Ebinop Oadd (Etempvar _t'2 tint) (Econst_int (Int.repr 1) tint)
+            tint) tint)))
+    (Sassign
+      (Efield
+        (Ederef (Etempvar _s (tptr (Tstruct _stack noattr)))
+          (Tstruct _stack noattr)) _top tint) (Etempvar _t'1 tint)))
+  (Sassign
+    (Ederef
+      (Ebinop Oadd
+        (Efield
+          (Ederef (Etempvar _s (tptr (Tstruct _stack noattr)))
+            (Tstruct _stack noattr)) _items
+          (tarray (tptr (Tstruct _node_t noattr)) 100)) (Etempvar _t'1 tint)
+        (tptr (tptr (Tstruct _node_t noattr))))
+      (tptr (Tstruct _node_t noattr)))
+    (Etempvar _item (tptr (Tstruct _node_t noattr)))))
+|}.
+
+Definition f_isEmpty := {|
+  fn_return := tint;
+  fn_callconv := cc_default;
+  fn_params := ((_s, (tptr (Tstruct _stack noattr))) :: nil);
+  fn_vars := nil;
+  fn_temps := ((_t'1, tint) :: nil);
+  fn_body :=
+(Ssequence
+  (Sset _t'1
+    (Efield
+      (Ederef (Etempvar _s (tptr (Tstruct _stack noattr)))
+        (Tstruct _stack noattr)) _top tint))
+  (Sreturn (Some (Ebinop Oeq (Etempvar _t'1 tint)
+                   (Eunop Oneg (Econst_int (Int.repr 1) tint) tint) tint))))
+|}.
+
+Definition f_pop := {|
+  fn_return := (tptr (Tstruct _node_t noattr));
+  fn_callconv := cc_default;
+  fn_params := ((_s, (tptr (Tstruct _stack noattr))) :: nil);
+  fn_vars := nil;
+  fn_temps := ((_t'2, tint) :: (_t'1, tint) ::
+               (_t'3, (tptr (Tstruct _node_t noattr))) :: nil);
+  fn_body :=
+(Ssequence
+  (Ssequence
+    (Scall (Some _t'2)
+      (Evar _isEmpty (Tfunction (Tcons (tptr (Tstruct _stack noattr)) Tnil)
+                       tint cc_default))
+      ((Etempvar _s (tptr (Tstruct _stack noattr))) :: nil))
+    (Sifthenelse (Eunop Onotbool (Etempvar _t'2 tint) tint)
+      (Ssequence
+        (Ssequence
+          (Sset _t'1
+            (Efield
+              (Ederef (Etempvar _s (tptr (Tstruct _stack noattr)))
+                (Tstruct _stack noattr)) _top tint))
+          (Sassign
+            (Efield
+              (Ederef (Etempvar _s (tptr (Tstruct _stack noattr)))
+                (Tstruct _stack noattr)) _top tint)
+            (Ebinop Osub (Etempvar _t'1 tint) (Econst_int (Int.repr 1) tint)
+              tint)))
+        (Ssequence
+          (Sset _t'3
+            (Ederef
+              (Ebinop Oadd
+                (Efield
+                  (Ederef (Etempvar _s (tptr (Tstruct _stack noattr)))
+                    (Tstruct _stack noattr)) _items
+                  (tarray (tptr (Tstruct _node_t noattr)) 100))
+                (Etempvar _t'1 tint) (tptr (tptr (Tstruct _node_t noattr))))
+              (tptr (Tstruct _node_t noattr))))
+          (Sreturn (Some (Etempvar _t'3 (tptr (Tstruct _node_t noattr)))))))
+      Sskip))
+  (Sreturn (Some (Ecast (Econst_int (Int.repr 0) tint) (tptr tvoid)))))
+|}.
+
+Definition f_insertOp_giveup := {|
+  fn_return := tvoid;
+  fn_callconv := cc_default;
+  fn_params := ((_p, (tptr (Tstruct _node_t noattr))) :: (_x, tint) ::
+                (_value, (tptr tvoid)) :: (_status, tint) :: nil);
+  fn_vars := ((_dlist, (Tstruct _DList noattr)) :: nil);
+  fn_temps := ((_l, (tptr (Tstruct _atom_int noattr))) ::
+               (_t'3, (tptr (Tstruct _atom_int noattr))) ::
+               (_t'2, (tptr tvoid)) :: (_t'1, (tptr tvoid)) ::
+               (_t'22, tulong) :: (_t'21, (tptr (tptr tvoid))) ::
+               (_t'20, (tptr tvoid)) :: (_t'19, (tptr (tptr tvoid))) ::
+               (_t'18, (tptr tvoid)) :: (_t'17, (tptr (tptr tvoid))) ::
+               (_t'16, (tptr tvoid)) :: (_t'15, (tptr (tptr tvoid))) ::
+               (_t'14, (tptr tvoid)) :: (_t'13, (tptr (tptr tvoid))) ::
+               (_t'12, (tptr (Tstruct _node noattr))) ::
+               (_t'11, (tptr tvoid)) :: (_t'10, (tptr (tptr tvoid))) ::
+               (_t'9, tint) :: (_t'8, (tptr tvoid)) ::
+               (_t'7, (tptr (tptr tvoid))) :: (_t'6, (tptr tvoid)) ::
+               (_t'5, (tptr (tptr tvoid))) :: (_t'4, (tptr (tptr tvoid))) ::
+               nil);
+  fn_body :=
+(Ssequence
+  (Sassign (Efield (Evar _dlist (Tstruct _DList noattr)) _size tulong)
+    (Econst_int (Int.repr 1) tint))
+  (Ssequence
+    (Ssequence
+      (Ssequence
+        (Sset _t'22
+          (Efield (Evar _dlist (Tstruct _DList noattr)) _size tulong))
+        (Scall (Some _t'1)
+          (Evar _surely_malloc (Tfunction (Tcons tulong Tnil) (tptr tvoid)
+                                 cc_default))
+          ((Ebinop Omul (Etempvar _t'22 tulong)
+             (Esizeof (tptr (Tstruct _node_t noattr)) tulong) tulong) :: nil)))
+      (Sassign
+        (Efield (Evar _dlist (Tstruct _DList noattr)) _list
+          (tptr (tptr tvoid)))
+        (Ecast (Etempvar _t'1 (tptr tvoid)) (tptr (tptr tvoid)))))
+    (Ssequence
+      (Ssequence
+        (Scall (Some _t'2)
+          (Evar _surely_malloc (Tfunction (Tcons tulong Tnil) (tptr tvoid)
+                                 cc_default))
+          ((Esizeof (Tstruct _node_t noattr) tulong) :: nil))
+        (Ssequence
+          (Sset _t'21
+            (Efield (Evar _dlist (Tstruct _DList noattr)) _list
+              (tptr (tptr tvoid))))
+          (Sassign
+            (Ederef
+              (Ebinop Oadd (Etempvar _t'21 (tptr (tptr tvoid)))
+                (Econst_int (Int.repr 0) tint) (tptr (tptr tvoid)))
+              (tptr tvoid))
+            (Ecast (Etempvar _t'2 (tptr tvoid)) (tptr tvoid)))))
+      (Ssequence
+        (Ssequence
+          (Scall (Some _t'3)
+            (Evar _makelock (Tfunction Tnil (tptr (Tstruct _atom_int noattr))
+                              cc_default)) nil)
+          (Sset _l (Etempvar _t'3 (tptr (Tstruct _atom_int noattr)))))
+        (Ssequence
+          (Ssequence
+            (Sset _t'19
+              (Efield (Evar _dlist (Tstruct _DList noattr)) _list
+                (tptr (tptr tvoid))))
+            (Ssequence
+              (Sset _t'20
+                (Ederef
+                  (Ebinop Oadd (Etempvar _t'19 (tptr (tptr tvoid)))
+                    (Econst_int (Int.repr 0) tint) (tptr (tptr tvoid)))
+                  (tptr tvoid)))
+              (Sassign
+                (Efield
+                  (Ederef
+                    (Ecast (Etempvar _t'20 (tptr tvoid))
+                      (tptr (Tstruct _node_t noattr)))
+                    (Tstruct _node_t noattr)) _lock
+                  (tptr (Tstruct _atom_int noattr)))
+                (Etempvar _l (tptr (Tstruct _atom_int noattr))))))
+          (Ssequence
+            (Scall None
+              (Evar _release (Tfunction
+                               (Tcons (tptr (Tstruct _atom_int noattr)) Tnil)
+                               tvoid cc_default))
+              ((Etempvar _l (tptr (Tstruct _atom_int noattr))) :: nil))
+            (Ssequence
+              (Sifthenelse (Ebinop Oeq (Etempvar _status tint)
+                             (Econst_int (Int.repr 2) tint) tint)
+                (Ssequence
+                  (Ssequence
+                    (Sset _t'17
+                      (Efield (Evar _dlist (Tstruct _DList noattr)) _list
+                        (tptr (tptr tvoid))))
+                    (Ssequence
+                      (Sset _t'18
+                        (Ederef
+                          (Ebinop Oadd (Etempvar _t'17 (tptr (tptr tvoid)))
+                            (Econst_int (Int.repr 0) tint)
+                            (tptr (tptr tvoid))) (tptr tvoid)))
+                      (Sassign
+                        (Efield
+                          (Ederef
+                            (Ecast (Etempvar _t'18 (tptr tvoid))
+                              (tptr (Tstruct _node_t noattr)))
+                            (Tstruct _node_t noattr)) _t
+                          (tptr (Tstruct _node noattr)))
+                        (Ecast (Econst_int (Int.repr 0) tint) (tptr tvoid)))))
+                  (Ssequence
+                    (Scall None
+                      (Evar _insertOp (Tfunction
+                                        (Tcons
+                                          (tptr (tptr (Tstruct _node noattr)))
+                                          (Tcons tint
+                                            (Tcons (tptr tvoid)
+                                              (Tcons tint
+                                                (Tcons
+                                                  (tptr (Tstruct _DList noattr))
+                                                  Tnil))))) tvoid cc_default))
+                      ((Eaddrof
+                         (Efield
+                           (Ederef
+                             (Etempvar _p (tptr (Tstruct _node_t noattr)))
+                             (Tstruct _node_t noattr)) _t
+                           (tptr (Tstruct _node noattr)))
+                         (tptr (tptr (Tstruct _node noattr)))) ::
+                       (Etempvar _x tint) ::
+                       (Etempvar _value (tptr tvoid)) ::
+                       (Etempvar _status tint) ::
+                       (Eaddrof (Evar _dlist (Tstruct _DList noattr))
+                         (tptr (Tstruct _DList noattr))) :: nil))
+                    (Ssequence
+                      (Ssequence
+                        (Sset _t'15
+                          (Efield (Evar _dlist (Tstruct _DList noattr)) _list
+                            (tptr (tptr tvoid))))
+                        (Ssequence
+                          (Sset _t'16
+                            (Ederef
+                              (Ebinop Oadd
+                                (Etempvar _t'15 (tptr (tptr tvoid)))
+                                (Econst_int (Int.repr 0) tint)
+                                (tptr (tptr tvoid))) (tptr tvoid)))
+                          (Sassign
+                            (Efield
+                              (Ederef
+                                (Ecast (Etempvar _t'16 (tptr tvoid))
+                                  (tptr (Tstruct _node_t noattr)))
+                                (Tstruct _node_t noattr)) _min tint)
+                            (Etempvar _x tint))))
+                      (Ssequence
+                        (Sset _t'13
+                          (Efield (Evar _dlist (Tstruct _DList noattr)) _list
+                            (tptr (tptr tvoid))))
+                        (Ssequence
+                          (Sset _t'14
+                            (Ederef
+                              (Ebinop Oadd
+                                (Etempvar _t'13 (tptr (tptr tvoid)))
+                                (Econst_int (Int.repr 0) tint)
+                                (tptr (tptr tvoid))) (tptr tvoid)))
+                          (Sassign
+                            (Efield
+                              (Ederef
+                                (Ecast (Etempvar _t'14 (tptr tvoid))
+                                  (tptr (Tstruct _node_t noattr)))
+                                (Tstruct _node_t noattr)) _max tint)
+                            (Econst_int (Int.repr 2147483647) tint)))))))
+                (Ssequence
+                  (Ssequence
+                    (Sset _t'10
+                      (Efield (Evar _dlist (Tstruct _DList noattr)) _list
+                        (tptr (tptr tvoid))))
+                    (Ssequence
+                      (Sset _t'11
+                        (Ederef
+                          (Ebinop Oadd (Etempvar _t'10 (tptr (tptr tvoid)))
+                            (Econst_int (Int.repr 0) tint)
+                            (tptr (tptr tvoid))) (tptr tvoid)))
+                      (Ssequence
+                        (Sset _t'12
+                          (Efield
+                            (Ederef
+                              (Etempvar _p (tptr (Tstruct _node_t noattr)))
+                              (Tstruct _node_t noattr)) _t
+                            (tptr (Tstruct _node noattr))))
+                        (Sassign
+                          (Efield
+                            (Ederef
+                              (Ecast (Etempvar _t'11 (tptr tvoid))
+                                (tptr (Tstruct _node_t noattr)))
+                              (Tstruct _node_t noattr)) _t
+                            (tptr (Tstruct _node noattr)))
+                          (Etempvar _t'12 (tptr (Tstruct _node noattr)))))))
+                  (Ssequence
+                    (Ssequence
+                      (Sset _t'7
+                        (Efield (Evar _dlist (Tstruct _DList noattr)) _list
+                          (tptr (tptr tvoid))))
+                      (Ssequence
+                        (Sset _t'8
+                          (Ederef
+                            (Ebinop Oadd (Etempvar _t'7 (tptr (tptr tvoid)))
+                              (Econst_int (Int.repr 0) tint)
+                              (tptr (tptr tvoid))) (tptr tvoid)))
+                        (Ssequence
+                          (Sset _t'9
+                            (Efield
+                              (Ederef
+                                (Etempvar _p (tptr (Tstruct _node_t noattr)))
+                                (Tstruct _node_t noattr)) _max tint))
+                          (Sassign
+                            (Efield
+                              (Ederef
+                                (Ecast (Etempvar _t'8 (tptr tvoid))
+                                  (tptr (Tstruct _node_t noattr)))
+                                (Tstruct _node_t noattr)) _max tint)
+                            (Etempvar _t'9 tint)))))
+                    (Ssequence
+                      (Ssequence
+                        (Sset _t'5
+                          (Efield (Evar _dlist (Tstruct _DList noattr)) _list
+                            (tptr (tptr tvoid))))
+                        (Ssequence
+                          (Sset _t'6
+                            (Ederef
+                              (Ebinop Oadd
+                                (Etempvar _t'5 (tptr (tptr tvoid)))
+                                (Econst_int (Int.repr 0) tint)
+                                (tptr (tptr tvoid))) (tptr tvoid)))
+                          (Sassign
+                            (Efield
+                              (Ederef
+                                (Ecast (Etempvar _t'6 (tptr tvoid))
+                                  (tptr (Tstruct _node_t noattr)))
+                                (Tstruct _node_t noattr)) _min tint)
+                            (Etempvar _x tint))))
+                      (Ssequence
+                        (Sassign
+                          (Efield
+                            (Ederef
+                              (Etempvar _p (tptr (Tstruct _node_t noattr)))
+                              (Tstruct _node_t noattr)) _t
+                            (tptr (Tstruct _node noattr)))
+                          (Ecast (Econst_int (Int.repr 0) tint) (tptr tvoid)))
+                        (Scall None
+                          (Evar _insertOp (Tfunction
+                                            (Tcons
+                                              (tptr (tptr (Tstruct _node noattr)))
+                                              (Tcons tint
+                                                (Tcons (tptr tvoid)
+                                                  (Tcons tint
+                                                    (Tcons
+                                                      (tptr (Tstruct _DList noattr))
+                                                      Tnil))))) tvoid
+                                            cc_default))
+                          ((Eaddrof
+                             (Efield
+                               (Ederef
+                                 (Etempvar _p (tptr (Tstruct _node_t noattr)))
+                                 (Tstruct _node_t noattr)) _t
+                               (tptr (Tstruct _node noattr)))
+                             (tptr (tptr (Tstruct _node noattr)))) ::
+                           (Etempvar _x tint) ::
+                           (Etempvar _value (tptr tvoid)) ::
+                           (Etempvar _status tint) ::
+                           (Eaddrof (Evar _dlist (Tstruct _DList noattr))
+                             (tptr (Tstruct _DList noattr))) :: nil)))))))
+              (Ssequence
+                (Sset _t'4
+                  (Efield (Evar _dlist (Tstruct _DList noattr)) _list
+                    (tptr (tptr tvoid))))
+                (Scall None
+                  (Evar _free (Tfunction (Tcons (tptr tvoid) Tnil) tvoid
+                                cc_default))
+                  ((Etempvar _t'4 (tptr (tptr tvoid))) :: nil))))))))))
+|}.
+
+Definition f_printDS_giveup := {|
+  fn_return := tvoid;
+  fn_callconv := cc_default;
+  fn_params := ((_t, (tptr (tptr tvoid))) :: nil);
+  fn_vars := ((_s, (Tstruct _stack noattr)) :: nil);
+  fn_temps := ((_tgt, (tptr (Tstruct _node_t noattr))) ::
+               (_current, (tptr (Tstruct _node_t noattr))) ::
+               (_t'3, (tptr (Tstruct _node_t noattr))) :: (_t'2, tint) ::
+               (_t'1, (tptr tvoid)) ::
+               (_t'6, (tptr (Tstruct _node noattr))) ::
+               (_t'5, (tptr (Tstruct _node noattr))) ::
+               (_t'4, (tptr (Tstruct _node noattr))) :: nil);
+  fn_body :=
+(Ssequence
+  (Scall None
+    (Evar _printf (Tfunction (Tcons (tptr tschar) Tnil) tint
+                    {|cc_vararg:=(Some 1); cc_unproto:=false; cc_structret:=false|}))
+    ((Evar ___stringlit_1 (tarray tschar 26)) :: nil))
+  (Ssequence
+    (Sset _tgt (Ederef (Etempvar _t (tptr (tptr tvoid))) (tptr tvoid)))
+    (Ssequence
+      (Sifthenelse (Ebinop Oeq
+                     (Etempvar _tgt (tptr (Tstruct _node_t noattr)))
+                     (Ecast (Econst_int (Int.repr 0) tint) (tptr tvoid))
+                     tint)
+        (Sreturn None)
+        Sskip)
+      (Ssequence
+        (Scall None
+          (Evar _initStack (Tfunction
+                             (Tcons (tptr (Tstruct _stack noattr)) Tnil)
+                             tvoid cc_default))
+          ((Eaddrof (Evar _s (Tstruct _stack noattr))
+             (tptr (Tstruct _stack noattr))) :: nil))
+        (Ssequence
+          (Sset _current (Etempvar _tgt (tptr (Tstruct _node_t noattr))))
+          (Ssequence
+            (Sloop
+              (Ssequence
+                (Ssequence
+                  (Sset _t'6
+                    (Efield
+                      (Ederef
+                        (Etempvar _current (tptr (Tstruct _node_t noattr)))
+                        (Tstruct _node_t noattr)) _t
+                      (tptr (Tstruct _node noattr))))
+                  (Sifthenelse (Ebinop One
+                                 (Etempvar _t'6 (tptr (Tstruct _node noattr)))
+                                 (Ecast (Econst_int (Int.repr 0) tint)
+                                   (tptr tvoid)) tint)
+                    Sskip
+                    Sbreak))
+                (Ssequence
+                  (Scall None
+                    (Evar _push (Tfunction
+                                  (Tcons (tptr (Tstruct _stack noattr))
+                                    (Tcons (tptr (Tstruct _node_t noattr))
+                                      Tnil)) tvoid cc_default))
+                    ((Eaddrof (Evar _s (Tstruct _stack noattr))
+                       (tptr (Tstruct _stack noattr))) ::
+                     (Etempvar _current (tptr (Tstruct _node_t noattr))) ::
+                     nil))
+                  (Ssequence
+                    (Ssequence
+                      (Sset _t'5
+                        (Efield
+                          (Ederef
+                            (Etempvar _current (tptr (Tstruct _node_t noattr)))
+                            (Tstruct _node_t noattr)) _t
+                          (tptr (Tstruct _node noattr))))
+                      (Scall (Some _t'1)
+                        (Evar _getNext (Tfunction
+                                         (Tcons (tptr (Tstruct _node noattr))
+                                           Tnil) (tptr tvoid) cc_default))
+                        ((Etempvar _t'5 (tptr (Tstruct _node noattr))) ::
+                         nil)))
+                    (Sset _current
+                      (Ecast (Etempvar _t'1 (tptr tvoid))
+                        (tptr (Tstruct _node_t noattr)))))))
+              Sskip)
+            (Sloop
+              (Ssequence
+                (Ssequence
+                  (Scall (Some _t'2)
+                    (Evar _isEmpty (Tfunction
+                                     (Tcons (tptr (Tstruct _stack noattr))
+                                       Tnil) tint cc_default))
+                    ((Eaddrof (Evar _s (Tstruct _stack noattr))
+                       (tptr (Tstruct _stack noattr))) :: nil))
+                  (Sifthenelse (Eunop Onotbool (Etempvar _t'2 tint) tint)
+                    Sskip
+                    Sbreak))
+                (Ssequence
+                  (Ssequence
+                    (Scall (Some _t'3)
+                      (Evar _pop (Tfunction
+                                   (Tcons (tptr (Tstruct _stack noattr))
+                                     Tnil) (tptr (Tstruct _node_t noattr))
+                                   cc_default))
+                      ((Eaddrof (Evar _s (Tstruct _stack noattr))
+                         (tptr (Tstruct _stack noattr))) :: nil))
+                    (Sset _current
+                      (Etempvar _t'3 (tptr (Tstruct _node_t noattr)))))
+                  (Ssequence
+                    (Sset _t'4
+                      (Efield
+                        (Ederef
+                          (Etempvar _current (tptr (Tstruct _node_t noattr)))
+                          (Tstruct _node_t noattr)) _t
+                        (tptr (Tstruct _node noattr))))
+                    (Scall None
+                      (Evar _printKey (Tfunction
+                                        (Tcons (tptr (Tstruct _node noattr))
+                                          Tnil) tvoid cc_default))
+                      ((Etempvar _t'4 (tptr (Tstruct _node noattr))) :: nil)))))
+              Sskip)))))))
+|}.
+
+Definition composites : list composite_definition :=
+(Composite _DList Struct
+   (Member_plain _list (tptr (tptr tvoid)) :: Member_plain _size tulong ::
+    nil)
+   noattr ::
+ Composite _node_t Struct
+   (Member_plain _t (tptr (Tstruct _node noattr)) ::
+    Member_plain _lock (tptr (Tstruct _atom_int noattr)) ::
+    Member_plain _min tint :: Member_plain _max tint :: nil)
+   noattr ::
+ Composite _stack Struct
+   (Member_plain _items (tarray (tptr (Tstruct _node_t noattr)) 100) ::
+    Member_plain _top tint :: nil)
+   noattr :: nil).
+
+Definition global_definitions : list (ident * globdef fundef type) :=
+((___compcert_va_int32,
+   Gfun(External (EF_runtime "__compcert_va_int32"
+                   (mksignature (AST.Tlong :: nil) AST.Tint cc_default))
+     (Tcons (tptr tvoid) Tnil) tuint cc_default)) ::
+ (___compcert_va_int64,
+   Gfun(External (EF_runtime "__compcert_va_int64"
+                   (mksignature (AST.Tlong :: nil) AST.Tlong cc_default))
+     (Tcons (tptr tvoid) Tnil) tulong cc_default)) ::
+ (___compcert_va_float64,
+   Gfun(External (EF_runtime "__compcert_va_float64"
+                   (mksignature (AST.Tlong :: nil) AST.Tfloat cc_default))
+     (Tcons (tptr tvoid) Tnil) tdouble cc_default)) ::
+ (___compcert_va_composite,
+   Gfun(External (EF_runtime "__compcert_va_composite"
+                   (mksignature (AST.Tlong :: AST.Tlong :: nil) AST.Tlong
+                     cc_default)) (Tcons (tptr tvoid) (Tcons tulong Tnil))
+     (tptr tvoid) cc_default)) ::
+ (___compcert_i64_dtos,
+   Gfun(External (EF_runtime "__compcert_i64_dtos"
+                   (mksignature (AST.Tfloat :: nil) AST.Tlong cc_default))
+     (Tcons tdouble Tnil) tlong cc_default)) ::
+ (___compcert_i64_dtou,
+   Gfun(External (EF_runtime "__compcert_i64_dtou"
+                   (mksignature (AST.Tfloat :: nil) AST.Tlong cc_default))
+     (Tcons tdouble Tnil) tulong cc_default)) ::
+ (___compcert_i64_stod,
+   Gfun(External (EF_runtime "__compcert_i64_stod"
+                   (mksignature (AST.Tlong :: nil) AST.Tfloat cc_default))
+     (Tcons tlong Tnil) tdouble cc_default)) ::
+ (___compcert_i64_utod,
+   Gfun(External (EF_runtime "__compcert_i64_utod"
+                   (mksignature (AST.Tlong :: nil) AST.Tfloat cc_default))
+     (Tcons tulong Tnil) tdouble cc_default)) ::
+ (___compcert_i64_stof,
+   Gfun(External (EF_runtime "__compcert_i64_stof"
+                   (mksignature (AST.Tlong :: nil) AST.Tsingle cc_default))
+     (Tcons tlong Tnil) tfloat cc_default)) ::
+ (___compcert_i64_utof,
+   Gfun(External (EF_runtime "__compcert_i64_utof"
+                   (mksignature (AST.Tlong :: nil) AST.Tsingle cc_default))
+     (Tcons tulong Tnil) tfloat cc_default)) ::
+ (___compcert_i64_sdiv,
+   Gfun(External (EF_runtime "__compcert_i64_sdiv"
+                   (mksignature (AST.Tlong :: AST.Tlong :: nil) AST.Tlong
+                     cc_default)) (Tcons tlong (Tcons tlong Tnil)) tlong
+     cc_default)) ::
+ (___compcert_i64_udiv,
+   Gfun(External (EF_runtime "__compcert_i64_udiv"
+                   (mksignature (AST.Tlong :: AST.Tlong :: nil) AST.Tlong
+                     cc_default)) (Tcons tulong (Tcons tulong Tnil)) tulong
+     cc_default)) ::
+ (___compcert_i64_smod,
+   Gfun(External (EF_runtime "__compcert_i64_smod"
+                   (mksignature (AST.Tlong :: AST.Tlong :: nil) AST.Tlong
+                     cc_default)) (Tcons tlong (Tcons tlong Tnil)) tlong
+     cc_default)) ::
+ (___compcert_i64_umod,
+   Gfun(External (EF_runtime "__compcert_i64_umod"
+                   (mksignature (AST.Tlong :: AST.Tlong :: nil) AST.Tlong
+                     cc_default)) (Tcons tulong (Tcons tulong Tnil)) tulong
+     cc_default)) ::
+ (___compcert_i64_shl,
+   Gfun(External (EF_runtime "__compcert_i64_shl"
+                   (mksignature (AST.Tlong :: AST.Tint :: nil) AST.Tlong
+                     cc_default)) (Tcons tlong (Tcons tint Tnil)) tlong
+     cc_default)) ::
+ (___compcert_i64_shr,
+   Gfun(External (EF_runtime "__compcert_i64_shr"
+                   (mksignature (AST.Tlong :: AST.Tint :: nil) AST.Tlong
+                     cc_default)) (Tcons tulong (Tcons tint Tnil)) tulong
+     cc_default)) ::
+ (___compcert_i64_sar,
+   Gfun(External (EF_runtime "__compcert_i64_sar"
+                   (mksignature (AST.Tlong :: AST.Tint :: nil) AST.Tlong
+                     cc_default)) (Tcons tlong (Tcons tint Tnil)) tlong
+     cc_default)) ::
+ (___compcert_i64_smulh,
+   Gfun(External (EF_runtime "__compcert_i64_smulh"
+                   (mksignature (AST.Tlong :: AST.Tlong :: nil) AST.Tlong
+                     cc_default)) (Tcons tlong (Tcons tlong Tnil)) tlong
+     cc_default)) ::
+ (___compcert_i64_umulh,
+   Gfun(External (EF_runtime "__compcert_i64_umulh"
+                   (mksignature (AST.Tlong :: AST.Tlong :: nil) AST.Tlong
+                     cc_default)) (Tcons tulong (Tcons tulong Tnil)) tulong
+     cc_default)) :: (___stringlit_1, Gvar v___stringlit_1) ::
+ (___builtin_bswap64,
+   Gfun(External (EF_builtin "__builtin_bswap64"
+                   (mksignature (AST.Tlong :: nil) AST.Tlong cc_default))
+     (Tcons tulong Tnil) tulong cc_default)) ::
+ (___builtin_bswap,
+   Gfun(External (EF_builtin "__builtin_bswap"
+                   (mksignature (AST.Tint :: nil) AST.Tint cc_default))
+     (Tcons tuint Tnil) tuint cc_default)) ::
+ (___builtin_bswap32,
+   Gfun(External (EF_builtin "__builtin_bswap32"
+                   (mksignature (AST.Tint :: nil) AST.Tint cc_default))
+     (Tcons tuint Tnil) tuint cc_default)) ::
+ (___builtin_bswap16,
+   Gfun(External (EF_builtin "__builtin_bswap16"
+                   (mksignature (AST.Tint :: nil) AST.Tint16unsigned
+                     cc_default)) (Tcons tushort Tnil) tushort cc_default)) ::
+ (___builtin_clz,
+   Gfun(External (EF_builtin "__builtin_clz"
+                   (mksignature (AST.Tint :: nil) AST.Tint cc_default))
+     (Tcons tuint Tnil) tint cc_default)) ::
+ (___builtin_clzl,
+   Gfun(External (EF_builtin "__builtin_clzl"
+                   (mksignature (AST.Tlong :: nil) AST.Tint cc_default))
+     (Tcons tulong Tnil) tint cc_default)) ::
+ (___builtin_clzll,
+   Gfun(External (EF_builtin "__builtin_clzll"
+                   (mksignature (AST.Tlong :: nil) AST.Tint cc_default))
+     (Tcons tulong Tnil) tint cc_default)) ::
+ (___builtin_ctz,
+   Gfun(External (EF_builtin "__builtin_ctz"
+                   (mksignature (AST.Tint :: nil) AST.Tint cc_default))
+     (Tcons tuint Tnil) tint cc_default)) ::
+ (___builtin_ctzl,
+   Gfun(External (EF_builtin "__builtin_ctzl"
+                   (mksignature (AST.Tlong :: nil) AST.Tint cc_default))
+     (Tcons tulong Tnil) tint cc_default)) ::
+ (___builtin_ctzll,
+   Gfun(External (EF_builtin "__builtin_ctzll"
+                   (mksignature (AST.Tlong :: nil) AST.Tint cc_default))
+     (Tcons tulong Tnil) tint cc_default)) ::
+ (___builtin_fabs,
+   Gfun(External (EF_builtin "__builtin_fabs"
+                   (mksignature (AST.Tfloat :: nil) AST.Tfloat cc_default))
+     (Tcons tdouble Tnil) tdouble cc_default)) ::
+ (___builtin_fabsf,
+   Gfun(External (EF_builtin "__builtin_fabsf"
+                   (mksignature (AST.Tsingle :: nil) AST.Tsingle cc_default))
+     (Tcons tfloat Tnil) tfloat cc_default)) ::
+ (___builtin_fsqrt,
+   Gfun(External (EF_builtin "__builtin_fsqrt"
+                   (mksignature (AST.Tfloat :: nil) AST.Tfloat cc_default))
+     (Tcons tdouble Tnil) tdouble cc_default)) ::
+ (___builtin_sqrt,
+   Gfun(External (EF_builtin "__builtin_sqrt"
+                   (mksignature (AST.Tfloat :: nil) AST.Tfloat cc_default))
+     (Tcons tdouble Tnil) tdouble cc_default)) ::
+ (___builtin_memcpy_aligned,
+   Gfun(External (EF_builtin "__builtin_memcpy_aligned"
+                   (mksignature
+                     (AST.Tlong :: AST.Tlong :: AST.Tlong :: AST.Tlong ::
+                      nil) AST.Tvoid cc_default))
+     (Tcons (tptr tvoid)
+       (Tcons (tptr tvoid) (Tcons tulong (Tcons tulong Tnil)))) tvoid
+     cc_default)) ::
+ (___builtin_sel,
+   Gfun(External (EF_builtin "__builtin_sel"
+                   (mksignature (AST.Tint :: nil) AST.Tvoid
+                     {|cc_vararg:=(Some 1); cc_unproto:=false; cc_structret:=false|}))
+     (Tcons tbool Tnil) tvoid
+     {|cc_vararg:=(Some 1); cc_unproto:=false; cc_structret:=false|})) ::
+ (___builtin_annot,
+   Gfun(External (EF_builtin "__builtin_annot"
+                   (mksignature (AST.Tlong :: nil) AST.Tvoid
+                     {|cc_vararg:=(Some 1); cc_unproto:=false; cc_structret:=false|}))
+     (Tcons (tptr tschar) Tnil) tvoid
+     {|cc_vararg:=(Some 1); cc_unproto:=false; cc_structret:=false|})) ::
+ (___builtin_annot_intval,
+   Gfun(External (EF_builtin "__builtin_annot_intval"
+                   (mksignature (AST.Tlong :: AST.Tint :: nil) AST.Tint
+                     cc_default)) (Tcons (tptr tschar) (Tcons tint Tnil))
+     tint cc_default)) ::
+ (___builtin_membar,
+   Gfun(External (EF_builtin "__builtin_membar"
+                   (mksignature nil AST.Tvoid cc_default)) Tnil tvoid
+     cc_default)) ::
+ (___builtin_va_start,
+   Gfun(External (EF_builtin "__builtin_va_start"
+                   (mksignature (AST.Tlong :: nil) AST.Tvoid cc_default))
+     (Tcons (tptr tvoid) Tnil) tvoid cc_default)) ::
+ (___builtin_va_arg,
+   Gfun(External (EF_builtin "__builtin_va_arg"
+                   (mksignature (AST.Tlong :: AST.Tint :: nil) AST.Tvoid
+                     cc_default)) (Tcons (tptr tvoid) (Tcons tuint Tnil))
+     tvoid cc_default)) ::
+ (___builtin_va_copy,
+   Gfun(External (EF_builtin "__builtin_va_copy"
+                   (mksignature (AST.Tlong :: AST.Tlong :: nil) AST.Tvoid
+                     cc_default))
+     (Tcons (tptr tvoid) (Tcons (tptr tvoid) Tnil)) tvoid cc_default)) ::
+ (___builtin_va_end,
+   Gfun(External (EF_builtin "__builtin_va_end"
+                   (mksignature (AST.Tlong :: nil) AST.Tvoid cc_default))
+     (Tcons (tptr tvoid) Tnil) tvoid cc_default)) ::
+ (___builtin_unreachable,
+   Gfun(External (EF_builtin "__builtin_unreachable"
+                   (mksignature nil AST.Tvoid cc_default)) Tnil tvoid
+     cc_default)) ::
+ (___builtin_expect,
+   Gfun(External (EF_builtin "__builtin_expect"
+                   (mksignature (AST.Tlong :: AST.Tlong :: nil) AST.Tlong
+                     cc_default)) (Tcons tlong (Tcons tlong Tnil)) tlong
+     cc_default)) ::
+ (___builtin_fence,
+   Gfun(External (EF_builtin "__builtin_fence"
+                   (mksignature nil AST.Tvoid cc_default)) Tnil tvoid
+     cc_default)) ::
+ (___builtin_cls,
+   Gfun(External (EF_builtin "__builtin_cls"
+                   (mksignature (AST.Tint :: nil) AST.Tint cc_default))
+     (Tcons tint Tnil) tint cc_default)) ::
+ (___builtin_clsl,
+   Gfun(External (EF_builtin "__builtin_clsl"
+                   (mksignature (AST.Tlong :: nil) AST.Tint cc_default))
+     (Tcons tlong Tnil) tint cc_default)) ::
+ (___builtin_clsll,
+   Gfun(External (EF_builtin "__builtin_clsll"
+                   (mksignature (AST.Tlong :: nil) AST.Tint cc_default))
+     (Tcons tlong Tnil) tint cc_default)) ::
+ (___builtin_fmadd,
+   Gfun(External (EF_builtin "__builtin_fmadd"
+                   (mksignature
+                     (AST.Tfloat :: AST.Tfloat :: AST.Tfloat :: nil)
+                     AST.Tfloat cc_default))
+     (Tcons tdouble (Tcons tdouble (Tcons tdouble Tnil))) tdouble
+     cc_default)) ::
+ (___builtin_fmsub,
+   Gfun(External (EF_builtin "__builtin_fmsub"
+                   (mksignature
+                     (AST.Tfloat :: AST.Tfloat :: AST.Tfloat :: nil)
+                     AST.Tfloat cc_default))
+     (Tcons tdouble (Tcons tdouble (Tcons tdouble Tnil))) tdouble
+     cc_default)) ::
+ (___builtin_fnmadd,
+   Gfun(External (EF_builtin "__builtin_fnmadd"
+                   (mksignature
+                     (AST.Tfloat :: AST.Tfloat :: AST.Tfloat :: nil)
+                     AST.Tfloat cc_default))
+     (Tcons tdouble (Tcons tdouble (Tcons tdouble Tnil))) tdouble
+     cc_default)) ::
+ (___builtin_fnmsub,
+   Gfun(External (EF_builtin "__builtin_fnmsub"
+                   (mksignature
+                     (AST.Tfloat :: AST.Tfloat :: AST.Tfloat :: nil)
+                     AST.Tfloat cc_default))
+     (Tcons tdouble (Tcons tdouble (Tcons tdouble Tnil))) tdouble
+     cc_default)) ::
+ (___builtin_fmax,
+   Gfun(External (EF_builtin "__builtin_fmax"
+                   (mksignature (AST.Tfloat :: AST.Tfloat :: nil) AST.Tfloat
+                     cc_default)) (Tcons tdouble (Tcons tdouble Tnil))
+     tdouble cc_default)) ::
+ (___builtin_fmin,
+   Gfun(External (EF_builtin "__builtin_fmin"
+                   (mksignature (AST.Tfloat :: AST.Tfloat :: nil) AST.Tfloat
+                     cc_default)) (Tcons tdouble (Tcons tdouble Tnil))
+     tdouble cc_default)) ::
+ (___builtin_debug,
+   Gfun(External (EF_external "__builtin_debug"
+                   (mksignature (AST.Tint :: nil) AST.Tvoid
+                     {|cc_vararg:=(Some 1); cc_unproto:=false; cc_structret:=false|}))
+     (Tcons tint Tnil) tvoid
+     {|cc_vararg:=(Some 1); cc_unproto:=false; cc_structret:=false|})) ::
+ (_printf,
+   Gfun(External (EF_external "printf"
+                   (mksignature (AST.Tlong :: nil) AST.Tint
+                     {|cc_vararg:=(Some 1); cc_unproto:=false; cc_structret:=false|}))
+     (Tcons (tptr tschar) Tnil) tint
+     {|cc_vararg:=(Some 1); cc_unproto:=false; cc_structret:=false|})) ::
+ (_malloc,
+   Gfun(External EF_malloc (Tcons tulong Tnil) (tptr tvoid) cc_default)) ::
+ (_free, Gfun(External EF_free (Tcons (tptr tvoid) Tnil) tvoid cc_default)) ::
+ (_exit,
+   Gfun(External (EF_external "exit"
+                   (mksignature (AST.Tint :: nil) AST.Tvoid cc_default))
+     (Tcons tint Tnil) tvoid cc_default)) ::
+ (_makelock,
+   Gfun(External (EF_external "makelock"
+                   (mksignature nil AST.Tlong cc_default)) Tnil
+     (tptr (Tstruct _atom_int noattr)) cc_default)) ::
+ (_release,
+   Gfun(External (EF_external "release"
+                   (mksignature (AST.Tlong :: nil) AST.Tvoid cc_default))
+     (Tcons (tptr (Tstruct _atom_int noattr)) Tnil) tvoid cc_default)) ::
+ (_thread_lock, Gvar v_thread_lock) ::
+ (_surely_malloc, Gfun(Internal f_surely_malloc)) ::
+ (_insertOp,
+   Gfun(External (EF_external "insertOp"
+                   (mksignature
+                     (AST.Tlong :: AST.Tint :: AST.Tlong :: AST.Tint ::
+                      AST.Tlong :: nil) AST.Tvoid cc_default))
+     (Tcons (tptr (tptr (Tstruct _node noattr)))
+       (Tcons tint
+         (Tcons (tptr tvoid)
+           (Tcons tint (Tcons (tptr (Tstruct _DList noattr)) Tnil))))) tvoid
+     cc_default)) ::
+ (_getNext,
+   Gfun(External (EF_external "getNext"
+                   (mksignature (AST.Tlong :: nil) AST.Tlong cc_default))
+     (Tcons (tptr (Tstruct _node noattr)) Tnil) (tptr tvoid) cc_default)) ::
+ (_printKey,
+   Gfun(External (EF_external "printKey"
+                   (mksignature (AST.Tlong :: nil) AST.Tvoid cc_default))
+     (Tcons (tptr (Tstruct _node noattr)) Tnil) tvoid cc_default)) ::
+ (_tb, Gvar v_tb) :: (_initStack, Gfun(Internal f_initStack)) ::
+ (_push, Gfun(Internal f_push)) :: (_isEmpty, Gfun(Internal f_isEmpty)) ::
+ (_pop, Gfun(Internal f_pop)) ::
+ (_insertOp_giveup, Gfun(Internal f_insertOp_giveup)) ::
+ (_printDS_giveup, Gfun(Internal f_printDS_giveup)) :: nil).
+
+Definition public_idents : list ident :=
+(_printDS_giveup :: _insertOp_giveup :: _tb :: _printKey :: _getNext ::
+ _insertOp :: _thread_lock :: _release :: _makelock :: _exit :: _free ::
+ _malloc :: _printf :: ___builtin_debug :: ___builtin_fmin ::
+ ___builtin_fmax :: ___builtin_fnmsub :: ___builtin_fnmadd ::
+ ___builtin_fmsub :: ___builtin_fmadd :: ___builtin_clsll ::
+ ___builtin_clsl :: ___builtin_cls :: ___builtin_fence ::
+ ___builtin_expect :: ___builtin_unreachable :: ___builtin_va_end ::
+ ___builtin_va_copy :: ___builtin_va_arg :: ___builtin_va_start ::
+ ___builtin_membar :: ___builtin_annot_intval :: ___builtin_annot ::
+ ___builtin_sel :: ___builtin_memcpy_aligned :: ___builtin_sqrt ::
+ ___builtin_fsqrt :: ___builtin_fabsf :: ___builtin_fabs ::
+ ___builtin_ctzll :: ___builtin_ctzl :: ___builtin_ctz :: ___builtin_clzll ::
+ ___builtin_clzl :: ___builtin_clz :: ___builtin_bswap16 ::
+ ___builtin_bswap32 :: ___builtin_bswap :: ___builtin_bswap64 ::
+ ___compcert_i64_umulh :: ___compcert_i64_smulh :: ___compcert_i64_sar ::
+ ___compcert_i64_shr :: ___compcert_i64_shl :: ___compcert_i64_umod ::
+ ___compcert_i64_smod :: ___compcert_i64_udiv :: ___compcert_i64_sdiv ::
+ ___compcert_i64_utof :: ___compcert_i64_stof :: ___compcert_i64_utod ::
+ ___compcert_i64_stod :: ___compcert_i64_dtou :: ___compcert_i64_dtos ::
+ ___compcert_va_composite :: ___compcert_va_float64 ::
+ ___compcert_va_int64 :: ___compcert_va_int32 :: nil).
+
+Definition prog : Clight.program := 
+  mkprogram composites global_definitions public_idents _main Logic.I.
+
+
