concurrency/Modular/templates/auth_ext.v
@@ -1,0 +1,37 @@
+(** Assorted auxiliary lemmas for authoritative RAs *)
+
+From iris.algebra Require Import excl auth gmap agree gset.
+From iris.proofmode Require Import tactics.
+From iris.heap_lang Require Import par.
+From iris.bi.lib Require Import fractional.
+Set Default Proof Using "All".
+
+Lemma auth_own_incl `{inG Σ (authR A)} `{!CmraDiscrete A} γ (x y: A) :
+  own γ (● x) ∗ own γ (◯ y) -∗ ⌜y ≼ x⌝.
+Proof.
+  rewrite -own_op. rewrite own_valid. iPureIntro.
+  rewrite auth_both_valid_discrete.
+  simpl. intros H1. destruct H1 as [z H2]. (*destruct H2 as [a Ha]. destruct Ha as [Ha Hb].*)
+  apply z.
+Qed.
+
+Lemma auth_excl_update `{inG Σ (authR (optionUR (exclR A)))} `{OfeDiscrete A} γ ys xs1 xs2 :
+  own γ (● (Excl' xs1)) -∗ own γ (◯ (Excl' xs2)) ==∗
+      own γ (● (Excl' ys)) ∗ own γ (◯ (Excl' ys)).
+Proof.
+  iIntros "Hγ● Hγ◯".
+  iMod (own_update_2 _ _ _ (● Excl' ys ⋅ ◯ Excl' ys)
+          with "Hγ● Hγ◯") as "[$$]".
+  { apply auth_update. apply option_local_update. apply exclusive_local_update. done. }
+  done.
+Qed.
+
+(*
+Lemma auth_agree  `{inG Σ (authR (optionUR (exclR A)))} `{OfeDiscrete A} γ xs ys :
+  own γ (● (Excl' xs)) -∗ own γ (◯ (Excl' ys)) -∗ ⌜xs = ys⌝.
+Proof.
+  iIntros "Hγ● Hγ◯". iPoseProof (own_valid_2 with "Hγ● Hγ◯") as "H".
+  iEval (rewrite auth_both_valid) in "H".
+      as %[<-%Excl_included%leibniz_equiv _]%auth_both_valid.
+Qed.
+*)
