concurrency/Modular/templates/data_struct.v
@@ -1,7 +1,10 @@
 Require Import VST.concurrency.conclib.
+
+Require Import VST.concurrency.conclib.
 Require Import VST.floyd.proofauto.
 Require Import VST.atomics.general_locks.
 Require Import Coq.Sets.Ensembles.
+Require Import bst.flows_ora.
 Require Import bst.puretree.
 (* Require Import bst.give_up_template. 
  Require Import bst.bst_inst. *)
