concurrency/Modular/templates/flows_ora.v
@@ -1,0 +1,52 @@
+From flows Require Import flows.
+From iris_ora Require Export ora.
+Local Arguments validN _ _ _ !_ /.
+Local Arguments valid _ _  !_ /.
+Local Arguments op _ _ _ !_ /.
+Local Arguments pcore _ _ !_ /.
+
+Section flows.
+  Local Instance flows_order: OraOrder flowintT := fun (a b: flowintT) => a = b \/ b = intUndef.
+  Lemma Increasing_flows : forall (a : flowintT ), Increasing a <-> a = ε \/ a = intUndef.
+  Proof.
+  split; intros Ha.
+  - specialize (Ha ε).
+    rewrite right_id in Ha.
+    inversion Ha; auto.
+  - intros ?; destruct Ha.
+    + subst a. rewrite left_id; hnf; auto. 
+    + hnf. subst a. right.
+      by rewrite (intComp_undef_op).
+  Qed.
+
+  Definition flows_ora_mixin : DORAMixin flowintT.
+  Proof. 
+    split; try apply _; try done.
+    - intros ???.
+      rewrite Increasing_flows.
+      destruct x; inversion H; auto.
+    - intros ???; inversion H; hnf; auto.
+    - intros ?????; inversion H; subst; eexists; split; eauto; hnf; [left|right]; auto.
+    - intros ?????; inversion H0; subst; auto; hnf; auto. 
+    - intros ????; inversion H; subst; hnf; [left | right]; auto; by pose proof (intComp_undef_op y). 
+    - intros ????; inversion H0; subst; [auto | contradiction].
+    - intros ???;
+      destruct cx; unfold pcore, flowintRAcore; destruct x; intros H0;
+      inversion H0; subst; try eauto.
+      destruct (int f0 ⋅ y);  eexists; split; try done; subst; hnf; [left | right]; eauto;
+      eexists.
+      + rewrite (intComp_undef_op y);
+        eexists; split; last first; eauto; hnf; auto.
+      + inversion H0; subst. inversion H2.
+      + rewrite (intComp_undef_op y).
+        eexists; split; eauto; hnf; auto.
+   Qed.
+  
+  Canonical Structure flowsR := discreteOra flowintT flows_ora_mixin.
+
+  Global Instance flows_ora_discrete : OraDiscrete flowintT.
+  Proof. apply discrete_ora_discrete. Qed.
+
+  Canonical Structure flowintUR : uora := Uora flowintT flowint_ucmra_mixin.
+
+End flows.
