concurrency/Modular/templates/inset_flows.v
@@ -1,0 +1,112 @@
+Require Import Coq.Numbers.NatInt.NZAddOrder.
+Set Default Proof Using "All".
+Require Export flows.flows flows.ccm flows.multiset_flows bst.keyset_ra.
+
+(** Flow interface cameras and auxiliary lemmas for inset flows
+  (used in the give-up template proof). *)
+
+Section inset_flows.
+
+Context `{Countable K}.
+
+Definition KS := @KS K _ _.
+
+(** Keysets of flow interfaces *)
+
+Definition keyset (I : multiset_flowint_ur K) n := dom (inf I n) ∖ dom (out I n).
+
+Lemma keyset_def : ∀ k I_n n, k ∈ inset K I_n n → ¬ in_outsets K k I_n
+  → k ∈ keyset I_n n.
+Proof.
+  intros ? ? ? k_in_inset k_not_in_outsets.
+  unfold keyset.
+  unfold inset in k_in_inset.
+  unfold in_outsets in k_not_in_outsets.
+  rewrite elem_of_difference.
+  naive_solver.
+Qed.
+
+(* The global invariant ϕ. *)
+Definition globalinv root I :=
+  ✓I
+  ∧ (root ∈ dom I)
+  ∧ closed K I
+  ∧ (∀ k, k ∈ KS → k ∈ inset K I root).
+
+(** Assorted lemmas about inset flows used in the template proofs *)
+
+Lemma globalinv_root_fp: ∀ I root, globalinv root I → root ∈ dom I.
+Proof.
+  intros I root Hglob. unfold globalinv in Hglob.
+  destruct Hglob as [H1 [H2 H3]]. done.
+Qed.
+
+Lemma contextualLeq_impl_globalinv : ∀ I I' root,
+    globalinv root I →
+    contextualLeq K_multiset I I' →
+    (∀ n, n ∈ dom I' ∖ dom I → inset K I' n = ∅) →
+    globalinv root I'.
+Proof.
+  intros ? ? ? GI CLeq InfI'.
+  unfold contextualLeq in CLeq.
+  unfold globalinv in GI.
+  destruct GI as (_ & DomR & OutI & InfI).
+  destruct CLeq as (VI & VI' & DS & InfR & OutR).
+  unfold closed in OutI.
+  unfold globalinv, closed.
+  repeat split.
+  - trivial.
+  - set_solver.
+  - intros.
+    destruct (decide (n ∈ dom I')).
+    * apply flowint_valid_unfold in VI'.
+      destruct VI' as [Ir' (I'_def & I'_disj & _)].
+      assert (out_map I' !!! n = 0%CCM).
+      { unfold out_map. rewrite I'_def.
+        assert (¬ (n ∈ dom (out_map I'))).
+        { unfold dom, flowint_dom in e.
+          naive_solver.
+        }
+        rewrite I'_def in H0.
+        rewrite nzmap_elem_of_dom_total in H0 *.
+        apply dec_stable in H0.
+        unfold out_map in H0. auto.
+      }
+      unfold outset, nzmap_dom, out.
+      rewrite H0. simpl.
+      rewrite dom_empty.
+      apply not_elem_of_empty.
+    * assert (n ∉ dom I) by set_solver.
+      pose proof (OutR n n0). 
+      unfold outset, multiset_flows.K_multiset, multiset_flows.K_multiset_ccm.
+      unfold K_multiset, K_multiset_ccm in H1. rewrite <- H1.
+      pose proof (OutI k n).
+      unfold outset in H2.
+      trivial. 
+  - intros.
+    (*destruct H2 as (H2 & _).*)
+    specialize (InfI k).
+    (*rewrite <- H0 in DomR.*)
+    specialize (InfR root DomR).
+    unfold inset.
+    unfold inset in InfR.
+    rewrite <- InfR.
+    apply InfI in H0.
+    trivial.
+Qed.
+
+Lemma globalinv_root_ins : ∀ I Ir root k,
+    globalinv root I ∧ Ir ≼ I ∧ dom Ir = {[root]} ∧ k ∈ KS
+    → k ∈ inset K Ir root.
+Proof.
+  intros I Ir root k ((Hv & _ & _ & Hl) & [I2 Hincl] & Hdom & kKS).
+  specialize (Hl k kKS). 
+  apply (inset_monotone I Ir I2 k root); try done.
+  set_solver.
+Qed.
+
+
+End inset_flows.
+
+Arguments keyset _ {_ _} _ _ : assert.
+Arguments globalinv _ {_ _} _ _ : assert.
