concurrency/Modular/templates/keyset_ra.v
@@ -1,0 +1,320 @@
+(** Camera definitions and proofs for the keyset RA. *)
+
+From iris.algebra Require Import gset.
+From iris.proofmode Require Import tactics.
+From iris.base_logic.lib Require Export iprop.
+From iris.base_logic.lib Require Export invariants.
+
+Set Default Proof Using "All".
+Require Export (*search_str*) bst.flows_ora bst.auth_ext.
+
+Section Search_Structure.
+
+(* The set of keys. *)
+Context `{Countable K}.
+
+(* The search structure operations *)
+Inductive dOp := searchOp | insertOp | deleteOp.
+
+(* Specification of a search structure operation *)
+Definition Ψ dop k (C: gsetO K) (C': gsetO K) (res: bool) :=
+  match dop with
+  | searchOp => C' = C ∧ (if res then k ∈ C else k ∉ C)
+  | insertOp => C' = C ∪ {[k]} ∧ (if res then k ∉ C else k ∈ C)
+  | deleteOp => C' = C ∖ {[k]} ∧ (if res then k ∈ C else k ∉ C)
+  end.
+
+Lemma Ψ_impl_C_in_K dop k C C' res (Ks: gset K) :
+  Ψ dop k C C' res → C ⊆ Ks → k ∈ Ks → C' ⊆ Ks.
+Proof.
+  intros HΨ ? ?. unfold Ψ in HΨ.
+  destruct dop.
+  - destruct HΨ as [HΨ _]. subst C'. done.
+  - destruct HΨ as [HΨ _]. set_solver.
+  - destruct HΨ as [HΨ _]. set_solver.
+Qed.
+
+End Search_Structure.
+
+Section keyset_ra.
+
+(* The set of keys. *)
+Context `{Countable K}.
+
+(* The keyspace is some arbitrary finite subset of K. *)
+Parameter KS : gset K.
+
+Inductive prodT :=
+  prod : gset K*gset K → prodT
+| prodTop : prodT
+| prodBot : prodT.
+
+Canonical Structure prodRAC := leibnizO prodT.
+
+Global Instance prodOp : Op prodT :=
+  λ p1 p2,
+  match p1, p2 with
+  | prod (K1, C1), prod (K2, C2) =>
+    if (decide(C1 ⊆ K1)) then
+      (if (decide(C2 ⊆ K2)) then
+         (if (decide (K1 ## K2)) then
+            (if (decide (C1 ## C2)) then (prod (K1 ∪ K2, C1 ∪ C2))
+             else prodTop)
+          else prodTop)
+       else prodTop)
+    else prodTop
+  | prodTop, _ => prodTop
+  | _, prodTop => prodTop
+  | p1, prodBot => p1
+  | prodBot, p2 => p2 end.
+  
+Global Instance prodValid : Valid prodT :=
+λ p, match p with
+       | prod (K, C) => C ⊆ K
+       | prodTop => False
+       | prodBot => True end.
+
+Global Instance prodCore : PCore prodT :=
+  λ p, Some prodBot.
+
+Global Instance prodUnit : Unit prodT := prodBot.
+
+Definition prodRA_mixin : RAMixin prodT.
+Proof.
+  split; try apply _; try done.
+  - (* Core is unique? *)
+    intros ? ? cx -> ?. exists cx. done.
+  - unfold op, prodOp. intros [] [] []; try (simpl; done).
+    case_eq p. intros g g0 Hp. case_eq p0. intros g1 g2 Hp0. case_eq p1. intros g3 g4 Hp1.
+    destruct (decide (g2 ⊆ g1)). destruct (decide (g4 ⊆ g3)). destruct (decide (g1 ## g3)).
+    destruct (decide (g2 ## g4)). destruct (decide (g0 ⊆ g)). destruct (decide (g2 ∪ g4 ⊆ g1 ∪ g3)).
+    destruct (decide (g ## g1 ∪ g3)). destruct (decide (g0 ## g2 ∪ g4)).
+    destruct (decide (g ## g1)). destruct (decide (g0 ## g2)). destruct (decide (g0 ∪ g2 ⊆ g ∪ g1)).
+    destruct (decide (g ∪ g1 ## g3)). destruct (decide (g0 ∪ g2 ## g4)). apply leibniz_equiv_iff.
+    assert (g ∪ (g1 ∪ g3) = g ∪ g1 ∪ g3). { set_solver. }
+    assert (g0 ∪ (g2 ∪ g4) = g0 ∪ g2 ∪ g4). { set_solver. }
+    rewrite H0. rewrite H1. reflexivity.
+    unfold not in n. exfalso. apply n. set_solver.
+    unfold not in n. exfalso. apply n. set_solver.
+    unfold not in n. exfalso. apply n. set_solver.
+    unfold not in n. exfalso. apply n. set_solver.
+    unfold not in n. exfalso. apply n. set_solver.
+    destruct (decide (g ## g1)). destruct (decide (g0 ## g2)). destruct (decide (g ∪ g1 ## g3)).
+    destruct (decide (g0 ∪ g2 ## g4)).
+    unfold not in n. exfalso. apply n. set_solver.
+    unfold not in n. exfalso. apply n. set_solver.
+    destruct (decide (g0 ∪ g2 ⊆ g ∪ g1)); try done. done. done.
+    destruct (decide (g ## g1)). destruct (decide (g0 ## g2)). destruct (decide (g0 ∪ g2 ⊆ g ∪ g1)).
+    destruct (decide (g ∪ g1 ## g3)). destruct (decide (g0 ∪ g2 ## g4)).
+    unfold not in n. exfalso. apply n. set_solver. done. done. done. done. done.
+    unfold not in n. exfalso. apply n. set_solver. done.
+    unfold not in n. exfalso. apply n. set_solver.
+    destruct (decide (g0 ⊆ g)). destruct (decide (g ## g1)); try done.
+    destruct (decide (g0 ## g2)). destruct (decide (g0 ∪ g2 ⊆ g ∪ g1)).
+    destruct (decide (g ∪ g1 ## g3)). unfold not in n. exfalso. apply n. set_solver.
+    done. done. done. done. destruct (decide (g0 ⊆ g)).
+    destruct (decide (g ## g1)). destruct (decide (g0 ## g2)).
+    destruct (decide (g0 ∪ g2 ⊆ g ∪ g1)). done. done. done. done. done.
+    destruct (decide (g0 ⊆ g)). done. done.
+    case_eq p. intros g g0 Hp. case_eq p0. intros g1 g2 Hp0. destruct (decide (g0 ⊆ g)).
+    destruct (decide (g2 ⊆ g1)). destruct (decide (g ## g1)).
+    destruct (decide (g0 ## g2)). done. done. done. done. done.
+    case_eq p. intros g g0 Hp. case_eq p0. intros g1 g2 Hp0. destruct (decide (g0 ⊆ g)).
+    destruct (decide (g2 ⊆ g1)). destruct (decide (g ## g1)).
+    destruct (decide (g0 ## g2)). done. done. done. done. done.
+    case_eq p; try done. case_eq p; try done. case_eq p; try done. case_eq p; try done.
+    case_eq p; try done. case_eq p; try done. case_eq p. intros g g0 Hp. case_eq p0. intros g1 g2 Hp0.
+    destruct (decide (g0 ⊆ g)). destruct (decide (g2 ⊆ g1)). destruct (decide (g ## g1)).
+    destruct (decide (g0 ## g2)). done. done. done. done. done.
+    case_eq p; try done. case_eq p; try done.
+  - unfold op, prodOp. intros [] []. case_eq p. intros g g0 Hp. case_eq p0. intros g1 g2 Hp0.
+    destruct (decide (g0 ⊆ g)); try done. destruct (decide (g2 ⊆ g1)); try done.
+    destruct (decide (g ## g1)). destruct (decide (g0 ## g2)). destruct (decide (g1 ## g)).
+    destruct (decide (g2 ## g0)). assert (g1 ∪ g = g ∪ g1 ∧ g2 ∪ g0 = g0 ∪ g2) as [H1 H2]. { set_solver. }
+    rewrite H1; rewrite H2. done. unfold not in n. exfalso. apply n. done.
+    unfold not in n. exfalso. apply n. done. destruct (decide (g1 ## g)). destruct (decide (g2 ## g0)).
+    unfold not in n. exfalso. apply n. done. done. done. destruct (decide (g1 ## g)).
+    unfold not in n. exfalso. apply n. done. done. destruct (decide (g2 ⊆ g1)); try done.
+    case_eq p; try done. case_eq p; try done. case_eq p; try done. done. done.
+    case_eq p; try done. done. done.
+  - unfold pcore, prodCore. intros x cx. intros Hx. inversion Hx.
+    unfold op, prodOp. destruct x; try done.
+  - unfold pcore, prodCore. intros x cx Hx. inversion Hx. done.
+  - intros x y cx Hxy HS. inversion HS. exists prodBot. split; try done. exists prodBot; done.
+  - unfold valid, prodValid. intros x y. destruct x. destruct p.
+    destruct y. destruct p. unfold op, prodOp. destruct (decide (g0 ⊆ g)).
+    destruct (decide (g2 ⊆ g1)). destruct (decide (g ## g1)). destruct (decide (g0 ## g2)).
+    intros. done. intros; done. intros; done. intros; done. intros; done.
+    unfold op, prodOp. intros; done. unfold op, prodOp. done. unfold op, prodOp. done.
+    destruct y. destruct p. unfold op, prodOp. done. unfold op, prodOp. done. unfold op, prodOp. done.
+Qed.
+
+Canonical Structure KsetRA := discreteR prodT prodRA_mixin.
+
+Global Instance prodRA_cmra_discrete : CmraDiscrete KsetRA.
+Proof. apply discrete_cmra_discrete. Qed.
+
+Lemma prod_ucmra_mixin : UcmraMixin prodT.
+Proof.
+  split; try apply _; try done. unfold LeftId. intros x. unfold ε, prodUnit.
+  unfold op, prodOp. destruct x; try done.
+Qed.
+
+Canonical Structure keysetUR : ucmra := Ucmra prodT prod_ucmra_mixin.
+
+Lemma auth_ks_included (a1 a2 b1 b2: gset K) :
+  ✓ prod (a1, b1) → ✓ prod (a2, b2) → prod (a1, b1) ≼ prod (a2, b2)
+  → (a1 = a2 ∧ b1 = b2) ∨
+    (∃ a0 b0, a2 = a1 ∪ a0 ∧ b2 = b1 ∪ b0 ∧ a1 ## a0 ∧ b1 ## b0 ∧ b1 ⊆ a1 ∧ b2 ⊆ a2 ∧ b0 ⊆ a0).
+Proof.
+  intros H1 H2 H0. destruct H0 as [z H0]. assert (✓ z). { apply (cmra_valid_op_r (prod (a1, b1))).
+  rewrite <- H0. done. } rewrite /(✓ prod (a1, b1)) /= in H1. rewrite /(✓ prod (a2, b2)) /= in H2.
+  destruct z.
+  - destruct p. rewrite /(✓ prod (g, g0)) /= in H3. rewrite /(⋅) /= in H0.
+    destruct (decide (b1 ⊆ a1)). destruct (decide (g0 ⊆ g)). destruct (decide (a1 ## g)).
+    destruct (decide (b1 ## g0)). right. exists g, g0. set_solver. inversion H0. inversion H0.
+    inversion H0. inversion H0.
+  - rewrite /(✓ prodTop) /= in H0. exfalso. done.
+  - rewrite /(⋅) /= in H0. inversion H0. left. done.
+Qed.
+
+Lemma auth_ks_local_update_insert K1 C Cn k:
+  ✓ prod (KS, C) ∧ ✓ prod (K1, Cn) ∧ k ∈ K1 ∧ k ∉ Cn ∧ k ∈ KS →
+  (prod (KS, C), prod (K1, Cn)) ~l~> (prod (KS, C ∪ {[k]}), prod (K1, Cn ∪ {[k]})).
+Proof.
+  intros [H1 [H2 [H3 [H4 HKS]]]]. apply local_update_discrete. intros z.
+  intros _. intros. split. rewrite /(✓ prod (KS, C ∪ {[k]})) /=.
+  rewrite /(cmra_valid KsetRA) /=. rewrite /(✓ prod (KS, C)) /= in H1.
+  set_solver. rewrite /(opM) /= in H0.
+  destruct z. rewrite /(opM) /=. destruct c. destruct p. rewrite /(op) /= in H0.
+  rewrite /(cmra_op KsetRA) /= in H0. destruct (decide (Cn ⊆ K1)).
+  destruct (decide (g0 ⊆ g)). destruct (decide (K1 ## g)). destruct (decide (Cn ## g0)).
+  inversion H0. rewrite /(op) /=. rewrite /(cmra_op KsetRA) /=. destruct (decide (Cn ∪ {[k]} ⊆ K1)).
+  destruct (decide (g0 ⊆ g)). destruct (decide (K1 ## g)). destruct (decide (Cn ∪ {[k]} ## g0)).
+  assert (Cn ∪ g0 ∪ {[k]} = Cn ∪ {[k]} ∪ g0). { set_solver. } rewrite H6. rewrite H5. done.
+  unfold not in n. exfalso. apply n. set_solver. unfold not in n. exfalso. apply n. set_solver.
+  unfold not in n. exfalso. apply n. set_solver. unfold not in n. exfalso. apply n. set_solver.
+  unfold not in n. exfalso. apply n. set_solver. unfold not in n. exfalso. apply n. set_solver.
+  unfold not in n. exfalso. apply n. set_solver. unfold not in n. exfalso. apply n. set_solver.
+  rewrite /(op) /= in H0. rewrite /(cmra_op KsetRA) /= in H0. inversion H0.
+  rewrite /(op) /= in H0. rewrite /(cmra_op KsetRA) /= in H0. inversion H0.
+  rewrite /(op) /=. rewrite /(cmra_op KsetRA) /=. done.
+  rewrite /(opM) /=. inversion H0. done.
+Qed.
+
+Lemma auth_ks_local_update_delete K1 C Cn k:
+            ✓ prod (KS, C) ∧ ✓ prod (K1, Cn) ∧ k ∈ K1 ∧ k ∈ Cn →
+           (prod (KS, C), prod (K1, Cn)) ~l~> (prod (KS, C ∖ {[k]}), prod (K1, Cn ∖ {[k]})).
+Proof.
+  intros [H1 [H2 [H3 H4]]]. apply local_update_discrete. intros z.
+  intros _. intros. split. rewrite /(✓ prod (KS, C ∖ {[k]})) /=.
+  rewrite /(cmra_valid KsetRA) /=. rewrite /(✓ prod (KS, C)) /= in H1.
+  set_solver. rewrite /(opM) /= in H0.
+  destruct z. rewrite /(opM) /=. destruct c. destruct p. rewrite /(op) /= in H0.
+  rewrite /(cmra_op KsetRA) /= in H0. destruct (decide (Cn ⊆ K1)).
+  destruct (decide (g0 ⊆ g)). destruct (decide (K1 ## g)). destruct (decide (Cn ## g0)).
+  inversion H. rewrite /(op) /=. rewrite /(cmra_op KsetRA) /=. destruct (decide (Cn ∖ {[k]} ⊆ K1)).
+  destruct (decide (g0 ⊆ g)). destruct (decide (K1 ## g)). destruct (decide (Cn ∖ {[k]} ## g0)).
+  assert (k ∉ g0). { set_solver. }
+  assert ((Cn ∪ g0) ∖ {[k]} = Cn ∖ {[k]} ∪ g0). { set_solver. } rewrite <- H6. inversion H0. done.
+  unfold not in n. exfalso. apply n. set_solver. unfold not in n. exfalso. apply n. set_solver.
+  unfold not in n. exfalso. apply n. set_solver. unfold not in n. exfalso. apply n. set_solver.
+  unfold not in n. exfalso. apply n. set_solver. unfold not in n. exfalso. apply n. set_solver.
+  unfold not in n. exfalso. apply n. set_solver. unfold not in n. exfalso. apply n. set_solver.
+  rewrite /(op) /= in H0. rewrite /(cmra_op KsetRA) /= in H0. inversion H0.
+  rewrite /(op) /= in H0. rewrite /(cmra_op KsetRA) /= in H0. inversion H0.
+  rewrite /(op) /=. rewrite /(cmra_op KsetRA) /=. done.
+  rewrite /(opM) /=. inversion H0. done.
+Qed.
+
+End keyset_ra.
+
+Arguments keysetUR _ {_ _}.
+
+Section keyset_updates.
+  Context `{Countable K}.
+
+  (** RA for pairs of keysets and contents *)
+
+  Class keysetG Σ := KeysetG { keyset_inG :> inG Σ (authUR (keysetUR K)) }.
+  Definition keysetΣ : gFunctors := #[GFunctor (authUR (keysetUR K))].
+
+  Global Instance subG_keysetΣ {Σ} : subG keysetΣ Σ → keysetG Σ.
+  Proof. solve_inG. Qed.
+
+  Context `{!keysetG Σ}.
+
+  (** Some useful lemmas  *)
+
+  Lemma keyset_valid γ_k Ks C:
+    own γ_k (◯ prod (Ks, C)) -∗ ⌜C ⊆ Ks⌝.
+  Proof.
+    iIntros "Hks".
+    iPoseProof (own_valid with "Hks") as "HvldCn".
+    iDestruct "HvldCn" as %HvldCn.
+    rewrite auth_frag_valid in HvldCn.
+    unfold valid, cmra_valid in HvldCn.
+    simpl in HvldCn. unfold ucmra_valid in HvldCn. simpl in HvldCn.
+      by iPureIntro.
+  Qed.
+
+  (** Ghost update of abstract search structure state *)
+      
+  Lemma ghost_update_keyset γ_k dop (k: K) Cn Cn' res K1 C:
+    ⊢ ⌜Ψ dop k Cn Cn' res⌝ ∗ own γ_k (● prod (KS, C)) ∗ own γ_k (◯ prod (K1, Cn))
+    ∗ ⌜Cn' ⊆ K1⌝ ∗ ⌜k ∈ K1⌝ ∗ ⌜k ∈ KS⌝
+    ==∗ ∃ C', ⌜Ψ dop k C C' res⌝ ∗ own γ_k (● prod (KS, C'))
+      ∗ own γ_k (◯ prod (K1, Cn')).
+  Proof.
+    iIntros "(#HΨ & Ha & Hf & % & % & HKS)". iPoseProof (auth_own_incl γ_k (prod (KS, C)) (prod (K1, Cn))
+                with "[$Ha $Hf]") as "%". iDestruct "HKS" as %HKS.
+    iPoseProof ((own_valid γ_k (● prod (KS, C))) with "Ha") as "%".
+    iPoseProof ((own_valid γ_k (◯ prod (K1, Cn))) with "Hf") as "%".
+    assert ((K1 = KS ∧ Cn = C) ∨
+            (∃ a0 b0, KS = K1 ∪ a0 ∧ C = Cn ∪ b0 ∧ K1 ## a0 ∧ Cn ## b0 ∧ Cn ⊆ K1 ∧ C ⊆ KS ∧ b0 ⊆ a0)) as Hs.
+    { apply (auth_ks_included K1 KS Cn C); try done. rewrite <- auth_frag_valid. done. apply auth_auth_valid. done. }
+    destruct Hs.
+    - iEval (unfold Ψ) in "HΨ". destruct H5. destruct dop.
+      + iDestruct "HΨ" as "%". destruct H7.
+        iModIntro. iExists C. iEval (rewrite <-H7) in "Hf". iFrame. unfold Ψ.
+        iPureIntro. split; try done. rewrite <-H6. done.
+      + iDestruct "HΨ" as "%". destruct H7. destruct res.
+        * iMod (own_update_2 γ_k (● prod (KS, C)) (◯ prod (K1, Cn))
+          (● prod (KS, C ∪ {[k]}) ⋅ ◯ prod (K1, Cn ∪ {[k]})) with "[Ha] [Hf]") as "(Ha & Hf)"; try done.
+          { apply auth_update. apply auth_ks_local_update_insert.
+            repeat split; try done. apply auth_auth_valid.  done. apply auth_frag_valid. done.  }
+          iModIntro. iExists (C ∪ {[k]}). iEval (rewrite H7). iFrame.
+          unfold Ψ. iPureIntro. split; try done. rewrite <-H6. done.
+        * assert (Cn' = Cn). { set_solver. } iModIntro. iExists C. iEval (rewrite <-H9) in "Hf".
+          iFrame. unfold Ψ. iPureIntro. rewrite <- H6. split; try done. rewrite H9 in H7. done.
+      + iDestruct "HΨ" as "%". destruct H7. destruct res.
+        * iMod (own_update_2 γ_k (● prod (KS, C)) (◯ prod (K1, Cn))
+          (● prod (KS, C ∖ {[k]}) ⋅ ◯ prod (K1, Cn ∖ {[k]})) with "[Ha] [Hf]") as "(Ha & Hf)"; try done.
+          { apply auth_update. apply auth_ks_local_update_delete. repeat split; try done. apply auth_auth_valid. done. apply auth_frag_valid. done. }
+          iModIntro. iExists (C ∖ {[k]}). iEval (rewrite H7). iFrame.
+          unfold Ψ. iPureIntro. split; try done. rewrite <-H6. done.
+        * assert (Cn' = Cn). { set_solver. } iModIntro. iExists C. iEval (rewrite <-H9) in "Hf".
+          iFrame. unfold Ψ. iPureIntro. rewrite <- H6. split; try done. rewrite H9 in H7. done.
+    - destruct H5 as [Ko [Co [H5 [H6 [H7 [H8 [H9 [H10 H11]]]]]]]]. destruct dop.
+      + iDestruct "HΨ" as "%". destruct H12.
+        iModIntro. iExists C. iEval (rewrite <-H12) in "Hf". iFrame. unfold Ψ.
+        iPureIntro. split; try done. destruct res; set_solver.
+      + iDestruct "HΨ" as "%". destruct H12. destruct res.
+        * iMod (own_update_2 γ_k (● prod (KS, C)) (◯ prod (K1, Cn))
+          (● prod (KS, C ∪ {[k]}) ⋅ ◯ prod (K1, Cn ∪ {[k]})) with "[Ha] [Hf]") as "(Ha & Hf)"; try done.
+          { apply auth_update. apply auth_ks_local_update_insert. split; try done. }
+          iModIntro. iExists (C ∪ {[k]}). iEval (rewrite H12). iFrame.
+          unfold Ψ. iPureIntro. split; try done. set_solver.
+        * assert (Cn' = Cn). { set_solver. } iModIntro. iExists C. iEval (rewrite <-H14) in "Hf".
+          iFrame. unfold Ψ. iPureIntro. set_solver.
+      + iDestruct "HΨ" as "%". destruct H12. destruct res.
+        * iMod (own_update_2 γ_k (● prod (KS, C)) (◯ prod (K1, Cn))
+          (● prod (KS, C ∖ {[k]}) ⋅ ◯ prod (K1, Cn ∖ {[k]})) with "[Ha] [Hf]") as "(Ha & Hf)"; try done.
+          { apply auth_update. apply auth_ks_local_update_delete. repeat split; try done. }
+          iModIntro. iExists (C ∖ {[k]}). iEval (rewrite H12). iFrame.
+          unfold Ψ. iPureIntro. split; try done. set_solver.
+        * assert (Cn' = Cn). { set_solver. } iModIntro. iExists C. iEval (rewrite <-H14) in "Hf".
+          iFrame. unfold Ψ. iPureIntro. set_solver.
+  Qed.
+
+End keyset_updates.
